OCL_Object_Model.thy
@@ -31,7 +31,7 @@ definition "oper_type op \<equiv>
     else Tuple (fmap_of_list (map (\<lambda>p. (param_name p, param_type p))
       (params @ [(STR ''result'', oper_result op, Out)])))"
 
-class ocl_object_model =
+class ocl_object_model' =
   fixes attributes :: "'a :: semilattice_sup \<rightharpoonup>\<^sub>f attr \<rightharpoonup>\<^sub>f 'a type"
   and associations :: "assoc \<rightharpoonup>\<^sub>f role \<rightharpoonup>\<^sub>f 'a assoc_end"
   and operations :: "('a type, 'a expr) oper_spec list"
@@ -45,6 +45,27 @@ abbreviation "find_association_end \<equiv> base.find_association_end"
 abbreviation "find_operation \<equiv> base.find_operation"
 abbreviation "find_static_operation \<equiv> base.find_static_operation"
 abbreviation "has_literal \<equiv> base.has_literal"
+
+end
+
+lemma find_implies_in_set:
+  "find P xs = Some x \<Longrightarrow> x \<in> set xs"
+  by (metis find_Some_iff nth_mem)
+
+lemma oper_type_wd:
+  "oper_result op \<noteq> OclInvalid \<Longrightarrow> oper_type op \<noteq> OclInvalid"
+  unfolding oper_type_def
+  apply auto
+  by (smt type.distinct(17))
+
+class ocl_object_model = ocl_object_model' +
+  assumes operations_wd: "\<And>op. op \<in> set operations \<Longrightarrow> oper_result op \<noteq> OclInvalid"
+begin
+
+lemma find_static_operation_wd:
+  "find_static_operation \<tau> op \<pi> = Some oper \<Longrightarrow>
+   oper_type oper \<noteq> OclInvalid"
+  by (simp add: operations_wd oper_type_wd find_implies_in_set)
 
 end
 
